@prefix dct: <http://purl.org/dc/terms/> .
@prefix prov: <http://www.w3.org/ns/prov#> .
@prefix rdfs: <http://www.w3.org/2000/01/rdf-schema#> .
@prefix schema: <https://schema.org/> .
@prefix skos: <http://www.w3.org/2004/02/skos/core#> .
@prefix surv: <https://linked.data.gov.au/def/csdm/surveyfeatures/> .
@prefix xsd: <http://www.w3.org/2001/XMLSchema#> .

<https://linked.data.gov.au/def/csdm/icsm-distance-type/3d-vector> a skos:Concept,
        surv:Distance ;
    skos:altLabel "Slope" ;
    skos:definition "The reduced observed slope distance between two survey marks." ;
    skos:inScheme <https://linked.data.gov.au/def/csdm/icsm-distance-type> ;
    skos:notation "3d-vector" ;
    skos:prefLabel "3D Vector" .

<https://linked.data.gov.au/def/csdm/icsm-distance-type/ellipsoid> a skos:Concept,
        surv:Distance ;
    skos:definition "The minimal length of a curve that joins two survey marks on a reference ellipsoid" ;
    skos:inScheme <https://linked.data.gov.au/def/csdm/icsm-distance-type> ;
    skos:notation "ellipsoid" ;
    skos:prefLabel "Ellipsoid" .

<https://linked.data.gov.au/def/csdm/icsm-distance-type/geodetic> a skos:Concept,
        surv:Distance ;
    skos:definition "The minimal length of a curve that joins two survey marks on a geodetic reference ellipsoid" ;
    skos:inScheme <https://linked.data.gov.au/def/csdm/icsm-distance-type> ;
    skos:notation "geodetic" ;
    skos:prefLabel "Geodetic" .

<https://linked.data.gov.au/def/csdm/icsm-distance-type/ground> a skos:Concept,
        surv:Distance ;
    skos:altLabel "G" ;
    skos:definition "The reduced observed distance between two survey marks at ground level" ;
    skos:inScheme <https://linked.data.gov.au/def/csdm/icsm-distance-type> ;
    skos:notation "ground" ;
    skos:prefLabel "Ground" .

<https://linked.data.gov.au/def/csdm/icsm-distance-type/horizontal> a skos:Concept,
        surv:Distance ;
    skos:definition "The reduced observed distance between two survey marks further reduced to a horizontal plane" ;
    skos:inScheme <https://linked.data.gov.au/def/csdm/icsm-distance-type> ;
    skos:notation "horizontal" ;
    skos:prefLabel "Horizontal" .

<https://linked.data.gov.au/def/csdm/icsm-distance-type/mean-elevation> a skos:Concept,
        surv:Distance ;
    skos:altLabel "Horizontal ground distance at mean elevation" ;
    skos:definition " The reduced observed horizontal distance between two survey marks adjusted to the mean elevation of the line measured" ;
    skos:inScheme <https://linked.data.gov.au/def/csdm/icsm-distance-type> ;
    skos:notation "mean-elevation" ;
    skos:prefLabel "Mean Elevation" .

<https://linked.data.gov.au/def/csdm/icsm-distance-type/slope> a skos:Concept,
        surv:Distance ;
    skos:definition "The reduced observed distance between two survey marks at ground level" ;
    skos:inScheme <https://linked.data.gov.au/def/csdm/icsm-distance-type> ;
    skos:notation "slope" ;
    skos:prefLabel "Slope" .

<https://linked.data.gov.au/def/csdm/icsm-distance-type/spheroid> a skos:Concept,
        surv:Distance ;
    skos:altLabel "S" ;
    skos:definition "The shortest distance between two points along the surface of a reference spheroid" ;
    skos:inScheme <https://linked.data.gov.au/def/csdm/icsm-distance-type> ;
    skos:notation "spheroid" ;
    skos:prefLabel "Spheroid" .

<https://linked.data.gov.au/def/csdm/icsm-distance-type> a skos:ConceptScheme ;
    skos:prefLabel "ICSM Distance Type" ;
    skos:scopeNote "surv:Distance" .

[] a prov:Activity ;
    prov:endedAtTime "2024-07-30T00:18:06.160119"^^xsd:dateTime ;
    prov:startedAtTime "2024-07-30T00:18:06.090447"^^xsd:dateTime ;
    prov:used [ a prov:Entity ;
            dct:format "application/json" ;
            dct:hasVersion "git:66a8ff4d5be1d1325924579f48173e14fea41ad0" ;
            rdfs:seeAlso <file:///home/runner/work/icsm-vocabs/icsm-vocabs/cadastre/SurveyObservations/icsm-distance-type.csv> ] ;
    prov:wasAssociatedWith [ a prov:Agent,
                schema:SoftwareApplication ;
            rdfs:label "OGC-NA tools" ;
            dct:hasVersion "0.3.49" ;
            rdfs:seeAlso <https://github.com/opengeospatial/ogc-na-tools> ] ;
    prov:wasInformedBy [ dct:identifier "7b8dc18d-b6bd-4abc-8ba5-d4554db0ca34" ] .

