@prefix dct: <http://purl.org/dc/terms/> .
@prefix prov: <http://www.w3.org/ns/prov#> .
@prefix rdfs: <http://www.w3.org/2000/01/rdf-schema#> .
@prefix schema: <https://schema.org/> .
@prefix skos: <http://www.w3.org/2004/02/skos/core#> .
@prefix sosa: <http://www.w3.org/ns/sosa/> .
@prefix xsd: <http://www.w3.org/2001/XMLSchema#> .

<https://linked.data.gov.au/def/csdm/icsm-procedure-used/adopted> a skos:Concept,
        sosa:Procedure ;
    skos:definition "The dimensions of the observation were adopted from a previous survey where the dimensions had been measured" ;
    skos:inScheme <https://linked.data.gov.au/def/csdm/icsm-procedure-used> ;
    skos:notation "adopted" ;
    skos:prefLabel "adopted" .

<https://linked.data.gov.au/def/csdm/icsm-procedure-used/approximate> a skos:Concept,
        sosa:Procedure ;
    skos:definition "Inaccurate - does not meet applicable standards of accuracy for cadastral surveys" ;
    skos:inScheme <https://linked.data.gov.au/def/csdm/icsm-procedure-used> ;
    skos:notation "approximate" ;
    skos:prefLabel "approximate" .

<https://linked.data.gov.au/def/csdm/icsm-procedure-used/calculated> a skos:Concept,
        sosa:Procedure ;
    skos:definition "Cadastral Boundaries created under the Operational Directives, such as Survey Registration Minute 1/98 and Executive Minutes 17/90 and 10/92 are to be shown as \"Calculated\".",
        "The dimensions of the observation where calculated" ;
    skos:inScheme <https://linked.data.gov.au/def/csdm/icsm-procedure-used> ;
    skos:notation "calculated" ;
    skos:prefLabel "Calculated",
        "calculated" .

<https://linked.data.gov.au/def/csdm/icsm-procedure-used/derived> a skos:Concept,
        sosa:Procedure ;
    skos:definition " Unsurveyed. Only applicable for mid azimuths and is derived from a mean of the reverse azimuths calculated from the two end points." ;
    skos:inScheme <https://linked.data.gov.au/def/csdm/icsm-procedure-used> ;
    skos:notation "derived" ;
    skos:prefLabel "derived" .

<https://linked.data.gov.au/def/csdm/icsm-procedure-used/described> a skos:Concept,
        sosa:Procedure ;
    skos:altLabel "metes & bounds" ;
    skos:definition "Unsurveyed. Directions and distances from physical monuments to define and describe the boundaries of the parcel. " ;
    skos:inScheme <https://linked.data.gov.au/def/csdm/icsm-procedure-used> ;
    skos:notation "described" ;
    skos:prefLabel "described" .

<https://linked.data.gov.au/def/csdm/icsm-procedure-used/measured> a skos:Concept,
        sosa:Procedure ;
    skos:definition "The dimensions of the observation were measured when the survey was conducted" ;
    skos:inScheme <https://linked.data.gov.au/def/csdm/icsm-procedure-used> ;
    skos:notation "measured" ;
    skos:prefLabel "measured" .

<https://linked.data.gov.au/def/csdm/icsm-procedure-used/scaled> a skos:Concept,
        sosa:Procedure ;
    skos:definition "The dimensions of the observation were scaled from a graphical plot" ;
    skos:inScheme <https://linked.data.gov.au/def/csdm/icsm-procedure-used> ;
    skos:notation "scaled" ;
    skos:prefLabel "scaled" .

<https://linked.data.gov.au/def/csdm/icsm-procedure-used> a skos:ConceptScheme ;
    skos:prefLabel "ICSM Survey Procedures" ;
    skos:scopeNote "sosa:Procedure" .

[] a prov:Activity ;
    prov:endedAtTime "2024-07-30T00:18:05.425026"^^xsd:dateTime ;
    prov:startedAtTime "2024-07-30T00:18:05.354739"^^xsd:dateTime ;
    prov:used [ a prov:Entity ;
            dct:format "application/json" ;
            dct:hasVersion "git:66a8ff4d5be1d1325924579f48173e14fea41ad0" ;
            rdfs:seeAlso <file:///home/runner/work/icsm-vocabs/icsm-vocabs/cadastre/SurveyObservations/icsm-procedure-used.csv> ] ;
    prov:wasAssociatedWith [ a prov:Agent,
                schema:SoftwareApplication ;
            rdfs:label "OGC-NA tools" ;
            dct:hasVersion "0.3.49" ;
            rdfs:seeAlso <https://github.com/opengeospatial/ogc-na-tools> ] ;
    prov:wasInformedBy [ dct:identifier "7b8dc18d-b6bd-4abc-8ba5-d4554db0ca34" ] .

