@prefix dct: <http://purl.org/dc/terms/> .
@prefix prov: <http://www.w3.org/ns/prov#> .
@prefix rdfs: <http://www.w3.org/2000/01/rdf-schema#> .
@prefix schema: <https://schema.org/> .
@prefix skos: <http://www.w3.org/2004/02/skos/core#> .
@prefix surv: <https://linked.data.gov.au/def/csdm/surveyfeatures/> .
@prefix xsd: <http://www.w3.org/2001/XMLSchema#> .

<https://linked.data.gov.au/def/csdm/icsm-angle-type/angle> a skos:Concept,
        surv:Angle ;
    skos:definition "The acute horizontal angle measured from a reference vector to the observed vector" ;
    skos:inScheme <https://linked.data.gov.au/def/csdm/icsm-angle-type> ;
    skos:notation "angle" ;
    skos:prefLabel "Angle" .

<https://linked.data.gov.au/def/csdm/icsm-angle-type/azimuth> a skos:Concept,
        surv:Angle ;
    skos:definition "The horizontal angle measured clockwise from any reference meridian to the observed vector" ;
    skos:inScheme <https://linked.data.gov.au/def/csdm/icsm-angle-type> ;
    skos:notation "azimuth" ;
    skos:prefLabel "Azimuth" .

<https://linked.data.gov.au/def/csdm/icsm-angle-type/bearing> a skos:Concept,
        surv:Angle ;
    skos:definition "The horizontal angle measured clockwise from the CRS meridian to the observed vector" ;
    skos:inScheme <https://linked.data.gov.au/def/csdm/icsm-angle-type> ;
    skos:notation "bearing" ;
    skos:prefLabel "Bearing" .

<https://linked.data.gov.au/def/csdm/icsm-angle-type/mid-azimuth> a skos:Concept,
        surv:Angle ;
    skos:definition "The mean of the forward azimuth at the start of the line and the reverse azimuth at the end of the line" ;
    skos:inScheme <https://linked.data.gov.au/def/csdm/icsm-angle-type> ;
    skos:notation "mid-azimuth" ;
    skos:prefLabel "Mid-azimuth" .

<https://linked.data.gov.au/def/csdm/icsm-angle-type/subtended> a skos:Concept,
        surv:Angle ;
    skos:definition "A subtended angle is an angle formed by two lines, or line segments that originate from the same point and extend to two different points on a circle's circumference." ;
    skos:inScheme <https://linked.data.gov.au/def/csdm/icsm-angle-type> ;
    skos:notation "subtended" ;
    skos:prefLabel "Subtended" .

<https://linked.data.gov.au/def/csdm/icsm-angle-type/v-angle> a skos:Concept,
        surv:Angle ;
    skos:definition "The vertical angle measured from the horizontal plane to the observed vector" ;
    skos:inScheme <https://linked.data.gov.au/def/csdm/icsm-angle-type> ;
    skos:notation "v-angle" ;
    skos:prefLabel "Vertical Angle" .

<https://linked.data.gov.au/def/csdm/icsm-angle-type> a skos:ConceptScheme ;
    skos:prefLabel "ICSM Angle Types" ;
    skos:scopeNote "surv:Angle" .

[] a prov:Activity ;
    prov:endedAtTime "2024-07-30T00:18:05.063988"^^xsd:dateTime ;
    prov:startedAtTime "2024-07-30T00:18:04.996197"^^xsd:dateTime ;
    prov:used [ a prov:Entity ;
            dct:format "application/json" ;
            dct:hasVersion "git:66a8ff4d5be1d1325924579f48173e14fea41ad0" ;
            rdfs:seeAlso <file:///home/runner/work/icsm-vocabs/icsm-vocabs/cadastre/SurveyObservations/icsm-angle-type.csv> ] ;
    prov:wasAssociatedWith [ a prov:Agent,
                schema:SoftwareApplication ;
            rdfs:label "OGC-NA tools" ;
            dct:hasVersion "0.3.49" ;
            rdfs:seeAlso <https://github.com/opengeospatial/ogc-na-tools> ] ;
    prov:wasInformedBy [ dct:identifier "7b8dc18d-b6bd-4abc-8ba5-d4554db0ca34" ] .

