@prefix dct: <http://purl.org/dc/terms/> .
@prefix prov: <http://www.w3.org/ns/prov#> .
@prefix rdfs: <http://www.w3.org/2000/01/rdf-schema#> .
@prefix schema: <https://schema.org/> .
@prefix skos: <http://www.w3.org/2004/02/skos/core#> .
@prefix termtype: <https://linked.data.gov.au/def/csdm/termtypes/> .
@prefix xsd: <http://www.w3.org/2001/XMLSchema#> .

<https://linked.data.gov.au/def/csdm/nz-vector-purpose/adopted> a skos:Concept,
        termtype:VectorPurpose ;
    skos:definition "The dimensions of the observation were adopted from a previous survey where the dimensions had been measured" ;
    skos:inScheme <https://linked.data.gov.au/def/csdm/nz-vector-purpose> ;
    skos:notation "adopted" ;
    skos:prefLabel "adopted" .

<https://linked.data.gov.au/def/csdm/nz-vector-purpose/calculated> a skos:Concept,
        termtype:VectorPurpose ;
    skos:definition "The dimensions of the observation where calculated" ;
    skos:inScheme <https://linked.data.gov.au/def/csdm/nz-vector-purpose> ;
    skos:notation "calculated" ;
    skos:prefLabel "calculated" .

<https://linked.data.gov.au/def/csdm/nz-vector-purpose/measured> a skos:Concept,
        termtype:VectorPurpose ;
    skos:definition "The dimensions of the observation were measured when the survey was conducted" ;
    skos:inScheme <https://linked.data.gov.au/def/csdm/nz-vector-purpose> ;
    skos:notation "measured" ;
    skos:prefLabel "measured" .

<https://linked.data.gov.au/def/csdm/nz-vector-purpose/pseudo> a skos:Concept,
        termtype:VectorPurpose ;
    skos:definition "The dimensions of the observation were calculated by Landonline from the coordinates of the local and remote setup's" ;
    skos:inScheme <https://linked.data.gov.au/def/csdm/nz-vector-purpose> ;
    skos:notation "pseudo" ;
    skos:prefLabel "pseudo" .

<https://linked.data.gov.au/def/csdm/nz-vector-purpose/reinadopted> a skos:Concept,
        termtype:VectorPurpose ;
    skos:altLabel "rein adopted" ;
    skos:definition "The dimensions of the observation were used for a reinstated boundary – no parcels are created" ;
    skos:inScheme <https://linked.data.gov.au/def/csdm/nz-vector-purpose> ;
    skos:notation "reinadopted" ;
    skos:prefLabel "reinadopted" .

<https://linked.data.gov.au/def/csdm/nz-vector-purpose/reincalculated> a skos:Concept,
        termtype:VectorPurpose ;
    skos:altLabel "rein calculated" ;
    skos:definition "The dimensions of the observation were used for a reinstated boundary – no parcels are created" ;
    skos:inScheme <https://linked.data.gov.au/def/csdm/nz-vector-purpose> ;
    skos:notation "reincalculated" ;
    skos:prefLabel "reincalculated" .

<https://linked.data.gov.au/def/csdm/nz-vector-purpose/scaled> a skos:Concept,
        termtype:VectorPurpose ;
    skos:altLabel "calculated" ;
    skos:definition "The dimensions of the observation were scaled from a graphical plot" ;
    skos:inScheme <https://linked.data.gov.au/def/csdm/nz-vector-purpose> ;
    skos:notation "scaled" ;
    skos:prefLabel "scaled" .

<https://linked.data.gov.au/def/csdm/nz-vector-purpose> a skos:ConceptScheme ;
    skos:prefLabel "NZ Vector Purpose" ;
    skos:scopeNote "termtype:VectorPurpose" .

[] a prov:Activity ;
    prov:endedAtTime "2024-07-30T00:18:05.698429"^^xsd:dateTime ;
    prov:startedAtTime "2024-07-30T00:18:05.629587"^^xsd:dateTime ;
    prov:used [ a prov:Entity ;
            dct:format "application/json" ;
            dct:hasVersion "git:66a8ff4d5be1d1325924579f48173e14fea41ad0" ;
            rdfs:seeAlso <file:///home/runner/work/icsm-vocabs/icsm-vocabs/cadastre/SurveyObservations/nz-vector-purpose.csv> ] ;
    prov:wasAssociatedWith [ a prov:Agent,
                schema:SoftwareApplication ;
            rdfs:label "OGC-NA tools" ;
            dct:hasVersion "0.3.49" ;
            rdfs:seeAlso <https://github.com/opengeospatial/ogc-na-tools> ] ;
    prov:wasInformedBy [ dct:identifier "7b8dc18d-b6bd-4abc-8ba5-d4554db0ca34" ] .

