@prefix dct: <http://purl.org/dc/terms/> .
@prefix prov: <http://www.w3.org/ns/prov#> .
@prefix rdfs: <http://www.w3.org/2000/01/rdf-schema#> .
@prefix schema: <https://schema.org/> .
@prefix skos: <http://www.w3.org/2004/02/skos/core#> .
@prefix termtype: <https://linked.data.gov.au/def/csdm/termtypes/> .
@prefix xsd: <http://www.w3.org/2001/XMLSchema#> .

<https://linked.data.gov.au/def/csdm/icsm-admin-unit-type/county> a skos:Concept,
        termtype:AdminUnitType ;
    skos:definition "A Victorian cadastral division for cadastral or land administration purposes" ;
    skos:inScheme <https://linked.data.gov.au/def/csdm/icsm-admin-unit-type> ;
    skos:notation "county" ;
    skos:prefLabel "County" .

<https://linked.data.gov.au/def/csdm/icsm-admin-unit-type/landDistrict> a skos:Concept,
        termtype:AdminUnitType ;
    skos:definition "A Land District is a NZ administrative area that all titles and surveys were registered against prior to Landonline." ;
    skos:inScheme <https://linked.data.gov.au/def/csdm/icsm-admin-unit-type> ;
    skos:notation "landDistrict" ;
    skos:prefLabel "Land District" .

<https://linked.data.gov.au/def/csdm/icsm-admin-unit-type/localGovernmentArea> a skos:Concept,
        termtype:AdminUnitType ;
    skos:altLabel "Local Government" ;
    skos:definition "Local government is the third level of government in Australia, administered with limited autonomy under the states and territories, and in turn beneath the federal government" ;
    skos:inScheme <https://linked.data.gov.au/def/csdm/icsm-admin-unit-type> ;
    skos:notation "localGovernmentArea" ;
    skos:prefLabel "Local Government Area" .

<https://linked.data.gov.au/def/csdm/icsm-admin-unit-type/locality> a skos:Concept,
        termtype:AdminUnitType ;
    skos:definition "A subdivision of a Western Australian Local Government Area" ;
    skos:inScheme <https://linked.data.gov.au/def/csdm/icsm-admin-unit-type> ;
    skos:notation "locality" ;
    skos:prefLabel "Locality" .

<https://linked.data.gov.au/def/csdm/icsm-admin-unit-type/parish> a skos:Concept,
        termtype:AdminUnitType ;
    skos:definition "A subdivision of a Victorian County" ;
    skos:inScheme <https://linked.data.gov.au/def/csdm/icsm-admin-unit-type> ;
    skos:notation "parish" ;
    skos:prefLabel "Parish" .

<https://linked.data.gov.au/def/csdm/icsm-admin-unit-type/territorialAuthority> a skos:Concept,
        termtype:AdminUnitType ;
    skos:altLabel "Municipality" ;
    skos:definition "A NZ territorial authority is defined under the Local Government Act 2002, NZ, as a city or a district council" ;
    skos:inScheme <https://linked.data.gov.au/def/csdm/icsm-admin-unit-type> ;
    skos:notation "territorialAuthority" ;
    skos:prefLabel "Territorial Authority" .

<https://linked.data.gov.au/def/csdm/icsm-admin-unit-type> a skos:ConceptScheme ;
    skos:prefLabel "ICSM Administrative Unit Types" ;
    skos:scopeNote "termtype:AdminUnitType" .

[] a prov:Activity ;
    prov:endedAtTime "2024-07-30T00:18:06.023236"^^xsd:dateTime ;
    prov:startedAtTime "2024-07-30T00:18:05.956492"^^xsd:dateTime ;
    prov:used [ a prov:Entity ;
            dct:format "application/json" ;
            dct:hasVersion "git:66a8ff4d5be1d1325924579f48173e14fea41ad0" ;
            rdfs:seeAlso <file:///home/runner/work/icsm-vocabs/icsm-vocabs/cadastre/CSD-Header/icsm-admin-unit-type.csv> ] ;
    prov:wasAssociatedWith [ a prov:Agent,
                schema:SoftwareApplication ;
            rdfs:label "OGC-NA tools" ;
            dct:hasVersion "0.3.49" ;
            rdfs:seeAlso <https://github.com/opengeospatial/ogc-na-tools> ] ;
    prov:wasInformedBy [ dct:identifier "7b8dc18d-b6bd-4abc-8ba5-d4554db0ca34" ] .

