@prefix dct: <http://purl.org/dc/terms/> .
@prefix prov: <http://www.w3.org/ns/prov#> .
@prefix rdfs: <http://www.w3.org/2000/01/rdf-schema#> .
@prefix schema: <https://schema.org/> .
@prefix skos: <http://www.w3.org/2004/02/skos/core#> .
@prefix termtype: <https://linked.data.gov.au/def/csdm/termtypes/> .
@prefix xsd: <http://www.w3.org/2001/XMLSchema#> .

<https://linked.data.gov.au/def/csdm/nz-survey-class/a> a skos:Concept,
        termtype:SurveyType ;
    skos:definition "Urban and the most accurate. The class A tolerance for boundary points increases from 0.06m at a rate of 0.015m per 100m." ;
    skos:inScheme <https://linked.data.gov.au/def/csdm/nz-survey-class> ;
    skos:notation "a" ;
    skos:prefLabel "Class A" .

<https://linked.data.gov.au/def/csdm/nz-survey-class/b> a skos:Concept,
        termtype:SurveyType ;
    skos:definition "Rural and not as accurate as class A. The class B tolerance for boundary points increases from 0.30m at a rate of 0.06m per 100m." ;
    skos:inScheme <https://linked.data.gov.au/def/csdm/nz-survey-class> ;
    skos:notation "b" ;
    skos:prefLabel "Class B" .

<https://linked.data.gov.au/def/csdm/nz-survey-class/c> a skos:Concept,
        termtype:SurveyType ;
    skos:definition "Used in specified rural circumstances where a less accurate boundary is acceptable. The class C tolerance for boundary points increases from 1.00m at a rate of 0.30m per 100m." ;
    skos:inScheme <https://linked.data.gov.au/def/csdm/nz-survey-class> ;
    skos:notation "c" ;
    skos:prefLabel "Class C" .

<https://linked.data.gov.au/def/csdm/nz-survey-class/d> a skos:Concept,
        termtype:SurveyType ;
    skos:definition "(used in exceptional circumstances where the existing boundary accuracy is unknown or unable to be determined and it is appropriate to permit these inaccuracies to remain" ;
    skos:inScheme <https://linked.data.gov.au/def/csdm/nz-survey-class> ;
    skos:notation "d" ;
    skos:prefLabel "Class D" .

<https://linked.data.gov.au/def/csdm/nz-survey-class> a skos:ConceptScheme ;
    skos:prefLabel "NZ Survey Class" ;
    skos:scopeNote "termtype:SurveyType" .

[] a prov:Activity ;
    prov:endedAtTime "2024-07-30T00:18:09.595310"^^xsd:dateTime ;
    prov:startedAtTime "2024-07-30T00:18:09.528660"^^xsd:dateTime ;
    prov:used [ a prov:Entity ;
            dct:format "application/json" ;
            dct:hasVersion "git:66a8ff4d5be1d1325924579f48173e14fea41ad0" ;
            rdfs:seeAlso <file:///home/runner/work/icsm-vocabs/icsm-vocabs/cadastre/CSD-Header/nz-survey-class.csv> ] ;
    prov:wasAssociatedWith [ a prov:Agent,
                schema:SoftwareApplication ;
            rdfs:label "OGC-NA tools" ;
            dct:hasVersion "0.3.49" ;
            rdfs:seeAlso <https://github.com/opengeospatial/ogc-na-tools> ] ;
    prov:wasInformedBy [ dct:identifier "7b8dc18d-b6bd-4abc-8ba5-d4554db0ca34" ] .

