@prefix dct: <http://purl.org/dc/terms/> .
@prefix prov: <http://www.w3.org/ns/prov#> .
@prefix rdfs: <http://www.w3.org/2000/01/rdf-schema#> .
@prefix schema: <https://schema.org/> .
@prefix skos: <http://www.w3.org/2004/02/skos/core#> .
@prefix surv: <https://linked.data.gov.au/def/csdm/surveyfeatures/> .
@prefix xsd: <http://www.w3.org/2001/XMLSchema#> .

<https://linked.data.gov.au/def/csdm/nz-monument-state/adpt> a skos:Concept,
        surv:SurveyPointState ;
    skos:altLabel "0" ;
    skos:definition "The mark existed before the survey was conducted and was adopted from a previous survey, i.e., It was not surveyed for this survey." ;
    skos:inScheme <https://linked.data.gov.au/def/csdm/nz-monument-state> ;
    skos:notation "adpt" ;
    skos:prefLabel "Adopted" .

<https://linked.data.gov.au/def/csdm/nz-monument-state/dist> a skos:Concept,
        surv:SurveyPointState ;
    skos:definition "The mark has been disturbed, hence a new coordinated position." ;
    skos:inScheme <https://linked.data.gov.au/def/csdm/nz-monument-state> ;
    skos:notation "dist" ;
    skos:prefLabel "Disturbed" .

<https://linked.data.gov.au/def/csdm/nz-monument-state/new> a skos:Concept,
        surv:SurveyPointState ;
    skos:altLabel "1" ;
    skos:definition "The mark was created by this survey." ;
    skos:inScheme <https://linked.data.gov.au/def/csdm/nz-monument-state> ;
    skos:notation "new" ;
    skos:prefLabel "New" .

<https://linked.data.gov.au/def/csdm/nz-monument-state/old> a skos:Concept,
        surv:SurveyPointState ;
    skos:altLabel "2" ;
    skos:definition "The mark existed before the survey was conducted. The mark is undisturbed and considered to be original. The mark was surveyed as part of this survey." ;
    skos:inScheme <https://linked.data.gov.au/def/csdm/nz-monument-state> ;
    skos:notation "old" ;
    skos:prefLabel "Old" .

<https://linked.data.gov.au/def/csdm/nz-monument-state/repl> a skos:Concept,
        surv:SurveyPointState ;
    skos:definition "The mark replaces an existing mark." ;
    skos:inScheme <https://linked.data.gov.au/def/csdm/nz-monument-state> ;
    skos:notation "repl" ;
    skos:prefLabel "Replaced" .

<https://linked.data.gov.au/def/csdm/nz-monument-state/sysa> a skos:Concept,
        surv:SurveyPointState ;
    skos:altLabel "3" ;
    skos:inScheme <https://linked.data.gov.au/def/csdm/nz-monument-state> ;
    skos:notation "sysa" ;
    skos:prefLabel "System Added" .

<https://linked.data.gov.au/def/csdm/nz-monument-state> a skos:ConceptScheme ;
    skos:prefLabel "NZ Monument State" ;
    skos:scopeNote "surv:SurveyPointState" .

[] a prov:Activity ;
    prov:endedAtTime "2024-07-30T00:18:09.526189"^^xsd:dateTime ;
    prov:startedAtTime "2024-07-30T00:18:09.455418"^^xsd:dateTime ;
    prov:used [ a prov:Entity ;
            dct:format "application/json" ;
            dct:hasVersion "git:66a8ff4d5be1d1325924579f48173e14fea41ad0" ;
            rdfs:seeAlso <file:///home/runner/work/icsm-vocabs/icsm-vocabs/cadastre/SurveyPoints/state/nz-state.csv> ] ;
    prov:wasAssociatedWith [ a prov:Agent,
                schema:SoftwareApplication ;
            rdfs:label "OGC-NA tools" ;
            dct:hasVersion "0.3.49" ;
            rdfs:seeAlso <https://github.com/opengeospatial/ogc-na-tools> ] ;
    prov:wasInformedBy [ dct:identifier "7b8dc18d-b6bd-4abc-8ba5-d4554db0ca34" ] .

