@prefix dct: <http://purl.org/dc/terms/> .
@prefix prov: <http://www.w3.org/ns/prov#> .
@prefix rdfs: <http://www.w3.org/2000/01/rdf-schema#> .
@prefix schema: <https://schema.org/> .
@prefix skos: <http://www.w3.org/2004/02/skos/core#> .
@prefix termtype: <https://linked.data.gov.au/def/csdm/termtypes/> .
@prefix xsd: <http://www.w3.org/2001/XMLSchema#> .

<https://linked.data.gov.au/def/csdm/nz-parcel-state/a> a skos:Concept,
        termtype:ParcelState ;
    skos:definition "The parcel must be amalgamated with one or more parcels created by the survey when the survey is deposited" ;
    skos:inScheme <https://linked.data.gov.au/def/csdm/nz-parcel-state> ;
    skos:notation "a" ;
    skos:prefLabel "affected" .

<https://linked.data.gov.au/def/csdm/nz-parcel-state/c> a skos:Concept,
        termtype:ParcelState ;
    skos:definition "The parcel is being created by the survey" ;
    skos:inScheme <https://linked.data.gov.au/def/csdm/nz-parcel-state> ;
    skos:notation "c" ;
    skos:prefLabel "created" .

<https://linked.data.gov.au/def/csdm/nz-parcel-state/enc> a skos:Concept,
        termtype:ParcelState ;
    skos:definition "The parcel has been subject to natural erosion and/or accretion and the definition of the parcel has been/should be updated. Relevant where the parcel affected by the accretion/erosion is not extinguished by the survey" ;
    skos:inScheme <https://linked.data.gov.au/def/csdm/nz-parcel-state> ;
    skos:notation "enc" ;
    skos:prefLabel "encroached" .

<https://linked.data.gov.au/def/csdm/nz-parcel-state/exist> a skos:Concept,
        termtype:ParcelState ;
    skos:definition "The parcel is referenced by the survey" ;
    skos:inScheme <https://linked.data.gov.au/def/csdm/nz-parcel-state> ;
    skos:notation "exist" ;
    skos:prefLabel "existing" .

<https://linked.data.gov.au/def/csdm/nz-parcel-state/exting> a skos:Concept,
        termtype:ParcelState ;
    skos:definition "The parcel is being replaced by one or more parcels created by the survey" ;
    skos:inScheme <https://linked.data.gov.au/def/csdm/nz-parcel-state> ;
    skos:notation "exting" ;
    skos:prefLabel "extinguished" .

<https://linked.data.gov.au/def/csdm/nz-parcel-state/prop> a skos:Concept,
        termtype:ParcelState ;
    skos:definition "The parcel is introduced on the survey but has not actually been ‘created’. This will generally only apply to parcels such as Future Development Units (FDU) on a Proposed Unit Development plan (PUD). The parcel will be created in a subsequent plan, e.g., Stage 1 of the Unit Development" ;
    skos:inScheme <https://linked.data.gov.au/def/csdm/nz-parcel-state> ;
    skos:notation "prop" ;
    skos:prefLabel "proposed" .

<https://linked.data.gov.au/def/csdm/nz-parcel-state/ref> a skos:Concept,
        termtype:ParcelState ;
    skos:definition "The parcel is referenced by the survey" ;
    skos:inScheme <https://linked.data.gov.au/def/csdm/nz-parcel-state> ;
    skos:notation "ref" ;
    skos:prefLabel "referenced" .

<https://linked.data.gov.au/def/csdm/nz-parcel-state> a skos:ConceptScheme ;
    skos:prefLabel "NZ Parcel State" ;
    skos:scopeNote "termtype:ParcelState" .

[] a prov:Activity ;
    prov:endedAtTime "2024-07-30T00:18:11.118218"^^xsd:dateTime ;
    prov:startedAtTime "2024-07-30T00:18:11.049397"^^xsd:dateTime ;
    prov:used [ a prov:Entity ;
            dct:format "application/json" ;
            dct:hasVersion "git:66a8ff4d5be1d1325924579f48173e14fea41ad0" ;
            rdfs:seeAlso <file:///home/runner/work/icsm-vocabs/icsm-vocabs/cadastre/Parcels/nz-parcel-state.csv> ] ;
    prov:wasAssociatedWith [ a prov:Agent,
                schema:SoftwareApplication ;
            rdfs:label "OGC-NA tools" ;
            dct:hasVersion "0.3.49" ;
            rdfs:seeAlso <https://github.com/opengeospatial/ogc-na-tools> ] ;
    prov:wasInformedBy [ dct:identifier "7b8dc18d-b6bd-4abc-8ba5-d4554db0ca34" ] .

