@prefix dct: <http://purl.org/dc/terms/> .
@prefix prov: <http://www.w3.org/ns/prov#> .
@prefix rdfs: <http://www.w3.org/2000/01/rdf-schema#> .
@prefix schema: <https://schema.org/> .
@prefix skos: <http://www.w3.org/2004/02/skos/core#> .
@prefix termtype: <https://linked.data.gov.au/def/csdm/termtypes/> .
@prefix xsd: <http://www.w3.org/2001/XMLSchema#> .

<https://linked.data.gov.au/def/csdm/vic-parcel-state/affected> a skos:Concept,
        termtype:ParcelState ;
    skos:definition "An existing parcel subject to amendment due to new boundary adoption from an abutting parcel" ;
    skos:inScheme <https://linked.data.gov.au/def/csdm/vic-parcel-state> ;
    skos:notation "affected" ;
    skos:prefLabel "Affected" .

<https://linked.data.gov.au/def/csdm/vic-parcel-state/cancelled> a skos:Concept,
        termtype:ParcelState ;
    skos:definition "An existing parcel subject to cancellation" ;
    skos:inScheme <https://linked.data.gov.au/def/csdm/vic-parcel-state> ;
    skos:notation "cancelled" ;
    skos:prefLabel "Cancelled" .

<https://linked.data.gov.au/def/csdm/vic-parcel-state/created> a skos:Concept,
        termtype:ParcelState ;
    skos:definition "A new parcel being created in a plan (e.g. (PS) plan of subdivision; (OP) original plan" ;
    skos:inScheme <https://linked.data.gov.au/def/csdm/vic-parcel-state> ;
    skos:notation "created" ;
    skos:prefLabel "Created" .

<https://linked.data.gov.au/def/csdm/vic-parcel-state/encroached> a skos:Concept,
        termtype:ParcelState ;
    skos:definition "An existing parcel encroached by a new boundary adoption from an abutting parcel" ;
    skos:inScheme <https://linked.data.gov.au/def/csdm/vic-parcel-state> ;
    skos:notation "encroached" ;
    skos:prefLabel "Encroached" .

<https://linked.data.gov.au/def/csdm/vic-parcel-state/existing> a skos:Concept,
        termtype:ParcelState ;
    skos:definition "A parcel that exists on the cadastre and the boundaries are not affected" ;
    skos:inScheme <https://linked.data.gov.au/def/csdm/vic-parcel-state> ;
    skos:notation "existing" ;
    skos:prefLabel "Existing" .

<https://linked.data.gov.au/def/csdm/vic-parcel-state/removed> a skos:Concept,
        termtype:ParcelState ;
    skos:definition "An easement / restriction subject to removal" ;
    skos:inScheme <https://linked.data.gov.au/def/csdm/vic-parcel-state> ;
    skos:notation "removed" ;
    skos:prefLabel "Removed" .

<https://linked.data.gov.au/def/csdm/vic-parcel-state> a skos:ConceptScheme ;
    skos:prefLabel "VIC Parcel State" ;
    skos:scopeNote "termtype:ParcelState" .

[] a prov:Activity ;
    prov:endedAtTime "2024-07-30T00:18:05.494988"^^xsd:dateTime ;
    prov:startedAtTime "2024-07-30T00:18:05.427609"^^xsd:dateTime ;
    prov:used [ a prov:Entity ;
            dct:format "application/json" ;
            dct:hasVersion "git:66a8ff4d5be1d1325924579f48173e14fea41ad0" ;
            rdfs:seeAlso <file:///home/runner/work/icsm-vocabs/icsm-vocabs/cadastre/Parcels/vic-parcel-state.csv> ] ;
    prov:wasAssociatedWith [ a prov:Agent,
                schema:SoftwareApplication ;
            rdfs:label "OGC-NA tools" ;
            dct:hasVersion "0.3.49" ;
            rdfs:seeAlso <https://github.com/opengeospatial/ogc-na-tools> ] ;
    prov:wasInformedBy [ dct:identifier "7b8dc18d-b6bd-4abc-8ba5-d4554db0ca34" ] .

